tactics: deprecate term_eq', rename to term_eq_old

src/tactics/FStar.Tactics.Basic.fst
@@ -1963,7 +1963,7 @@ let comp_to_string (c:comp) : tac string
   = let s = Print.comp_to_string c in
     ret s
 
-let term_eq' (t1:term) (t2:term) : tac bool
+let term_eq_old (t1:term) (t2:term) : tac bool
   = bind idtac (fun () ->
     ret (Syntax.Util.term_eq t1 t2))
 
