ulib/experimental/FStar.InteractiveHelpers.PostProcess.fst
@@ -13,7 +13,7 @@ open FStar.InteractiveHelpers.Propositions
 open FStar.InteractiveHelpers.Effectful
 open FStar.InteractiveHelpers.Output
 
-let term_eq = FStar.Tactics.term_eq'
+let term_eq = FStar.Tactics.term_eq_old
 
 /// The high-level post-processing tactics, used to retrieve some specific
 /// information from the context and generate output which can be exploited
