ulib/experimental/FStar.InteractiveHelpers.Propositions.fst
@@ -6,7 +6,7 @@ open FStar.Mul
 open FStar.InteractiveHelpers.Base
 open FStar.InteractiveHelpers.ExploreTerm
 
-let term_eq = FStar.Tactics.term_eq'
+let term_eq = FStar.Tactics.term_eq_old
 
 /// Propositions and assertions.
 /// Assertions are propositions to be inserted in the F* code: we differentiate
